{
 "cells": [
  {
   "cell_type": "code",
   "execution_count": 1,
   "id": "12a78e12",
   "metadata": {},
   "outputs": [
    {
     "name": "stdout",
     "output_type": "stream",
     "text": [
      "T(2) = 105\n"
     ]
    }
   ],
   "source": [
    "# 1. Find the value of T(2) for the recurrence relation T(n) = 3T(n-1) + 12n, given that T(0)=5.\n",
    "def recurrence_relation(n):\n",
    "    if n == 0:\n",
    "        return 5\n",
    "    else:\n",
    "        return 3 * recurrence_relation(n - 1) + 12 * n\n",
    "\n",
    "result = recurrence_relation(2)\n",
    "\n",
    "print(\"T(2) =\", result)"
   ]
  },
  {
   "cell_type": "markdown",
   "id": "ebd9946c",
   "metadata": {},
   "source": [
    "# 2. Given a recurrence relation, solve it using the substitution method:\n",
    "# a. T(n) = T(n-1) + c\n",
    "\n",
    "To solve the recurrence relation T(n) = T(n-1) + c using the substitution method, we'll first guess the form of the solution and then prove it by induction.\n",
    "\n",
    "Let's assume T(n) = an + b, where 'a' and 'b' are constants to be determined.\n",
    "\n",
    "Substituting this assumed form into the recurrence relation:\n",
    "\n",
    "an + b = a(n - 1) + b + c\n",
    "\n",
    "Expanding and simplifying:\n",
    "\n",
    "an + b = an - a + b + c\n",
    "\n",
    "Rearranging terms:\n",
    "\n",
    "c = -a\n",
    "\n",
    "Hence, we find that a = -c.\n",
    "\n",
    "Substituting a = -c back into our assumed form of the solution, we get:\n",
    "\n",
    "T(n) = -cn + b\n",
    "\n",
    "Now, let's verify this solution by induction.\n",
    "\n",
    "Base Case: For n = 1, T(1) = -c(1) + b = b - c, which satisfies the base case.\n",
    "\n",
    "Inductive Step: Assume that T(k) = -ck + b holds for some arbitrary k ≥ 1.\n",
    "\n",
    "Now, let's prove that T(k+1) = -c(k+1) + b holds:\n",
    "\n",
    "T(k+1) = T(k) + c = (-ck + b) + c = -c(k+1) + b\n",
    "\n",
    "Thus, the assumed solution T(n) = -cn + b satisfies the recurrence relation T(n) = T(n-1) + c for all n ≥ 1.\n",
    "\n",
    "Therefore, the solution to the recurrence relation T(n) = T(n-1) + c using the substitution method is T(n) = -cn + b, where b is an arbitrary constant."
   ]
  },
  {
   "cell_type": "markdown",
   "id": "e7814101",
   "metadata": {},
   "source": [
    "Solution of T(n) = T(n-1) + c using the substitution method\n",
    "\n",
    "This problem requires solving the recurrence relation T(n) = T(n-1) + c using the substitution method. We make an assumption about the form of the solution, substitute it into the recurrence relation, and then verify it through induction to determine the constants involved in the solution.\n",
    "\n",
    "Here's the explanation step by step:\n",
    "\n",
    "1. **Assumption of Solution Form**:\n",
    "   We assume a solution form for T(n) as \"an + b\", where 'a' and 'b' are constants to be determined.\n",
    "\n",
    "2. **Substitution into Recurrence Relation**:\n",
    "   We substitute this assumed form into the given recurrence relation T(n) = T(n-1) + c.\n",
    "\n",
    "3. **Expanding and Simplifying**:\n",
    "   After substituting, we expand and simplify the equation to get \"an + b = an - a + b + c\".\n",
    "\n",
    "4. **Rearranging Terms**:\n",
    "   Rearranging terms, we find that \"c = -a\". Thus, we determine that \"a = -c\".\n",
    "\n",
    "5. **Substituting Back**:\n",
    "   We substitute \"a = -c\" back into our assumed form of the solution, yielding \"T(n) = -cn + b\".\n",
    "\n",
    "6. **Verification -y Induction**:\n",
    "   - **Base Case**:\n",
    "       We check the base case for n = 1, which satisf-es T(1) = b - c.\n",
    "   - **Inductive Step**:\n",
    "       We assume T(k) = -ck + b holds for some arbitrary k ≥ 1, then prove that T(k+1) = -c(k+1) + b holds.\n",
    "\n",
    "7. **Conclusion**:\n",
    "   By verifying the base case and the inductive step, we conclude that the assumed solution T(n) = -cn + b satisfies the given recurrence relation for all n ≥ 1.\n",
    "e relation for all n ≥ 1.\n",
    "relation for all n ≥ 1.\n"
   ]
  },
  {
   "cell_type": "markdown",
   "id": "f3c84f82",
   "metadata": {},
   "source": [
    "# 2. Given a recurrence relation, solve it using the substitution method:\n",
    "# b. T(n) = 2T(n/2) + n\n",
    "\n",
    "To solve the recurrence relation T(n) = 2T(n/2) + n using the substitution method:\n",
    "\n",
    "Let's assume T(n) = anlog(n) + bn, where 'a' and 'b' are constants to be determined.\n",
    "\n",
    "Substituting this assumed form into the recurrence relation:\n",
    "\n",
    "anlog(n) + bn = 2a(n/2)log(n/2) + 2b(n/2) + n\n",
    "\n",
    "anlog(n) + bn = a(nlog(n) - nlog(2)) + 2b(n/2) + n\n",
    "\n",
    "anlog(n) + bn = a(nlog(n) - n) + bn + n\n",
    "\n",
    "anlog(n) + bn = anlog(n) - an + bn + n\n",
    "\n",
    "0 = -an + bn + n\n",
    "\n",
    "0 = (b-a)n + n\n",
    "\n",
    "0 = (b - a + 1)n\n",
    "\n",
    "This implies b - a + 1 = 0, therefore b = a - 1.\n",
    "\n",
    "Substituting b = a - 1 back into our assumed form of the solution, we get:\n",
    "\n",
    "T(n) = anlog(n) + (a - 1)n\n",
    "\n",
    "Now, let's verify this solution by induction.\n",
    "\n",
    "Base Case:\n",
    "For n = 1:\n",
    "T(1) = a(1)log(1) + (a - 1)(1) = 0\n",
    "\n",
    "Inductive Step:\n",
    "Assume that T(k) = aklog(k) + (a - 1)k holds for some arbitrary k ≥ 1.\n",
    "\n",
    "Now, let's prove that T(2k) = a(2k)log(2k) + (a - 1)(2k) holds:\n",
    "T(2k) = 2a(k)log(k) + (a - 1)(2k) + 2k\n",
    "\n",
    "T(2k) = 2aklog(k) + 2k(a - 1) + 2k\n",
    "\n",
    "T(2k) = 2aklog(k) + 2ka - 2k + 2k\n",
    "\n",
    "T(2k) = 2aklog(k) + 2ka\n",
    "\n",
    "T(2k) = 2aklog(2k) + 2ka\n",
    "\n",
    "Thus, the assumed solution T(n) = anlog(n) + (a - 1)n satisfies the recurrence relation T(n) = 2T(n/2) + n for all n ≥ 1.\n",
    "\n",
    "Therefore, the solution to the recurrence relation T(n) = 2T(n/2) + n using the substitution method is T(n) = anlog(n) + (a - 1)n, where a is an arbitrary constant."
   ]
  },
  {
   "cell_type": "markdown",
   "id": "bf96aadb",
   "metadata": {},
   "source": [
    "# 2. Given a recurrence relation, solve it using the substitution method:\n",
    "# c. T(n) = 2T(n/2) + c\n",
    "\n",
    "To solve the recurrence relation T(n) = 2T(n/2) + c using the substitution method:\n",
    "\n",
    "Let's assume T(n) = an + b, where 'a' and 'b' are constants to be determined.\n",
    "\n",
    "Substituting this assumed form into the recurrence relation:\n",
    "\n",
    "an + b = 2a(n/2) + b + c\n",
    "\n",
    "an + b = an + b + c\n",
    "\n",
    "Rearranging terms:\n",
    "\n",
    "c = 0\n",
    "\n",
    "This implies that 'c' must be equal to zero for the equation to hold.\n",
    "\n",
    "Substituting c = 0 back into our assumed form of the solution, we get:\n",
    "\n",
    "T(n) = an + b\n",
    "\n",
    "Now, let's verify this solution by induction.\n",
    "\n",
    "Base Case:\n",
    "For n = 1:\n",
    "T(1) = a(1) + b = a + b\n",
    "\n",
    "Inductive Step:\n",
    "Assume that T(k) = ak + b holds for some arbitrary k ≥ 1.\n",
    "\n",
    "Now, let's prove that T(2k) = a(2k) + b holds:\n",
    "T(2k) = 2a(k) + b\n",
    "\n",
    "T(2k) = 2ak + b\n",
    "\n",
    "T(2k) = a(2k) + b\n",
    "\n",
    "Thus, the assumed solution T(n) = an + b satisfies the recurrence relation T(n) = 2T(n/2) + c for all n ≥ 1, given that c = 0.\n",
    "\n",
    "Therefore, the solution to the recurrence relation T(n) = 2T(n/2) + c using the substitution method is T(n) = an + b, where 'a' and 'b' are arbitrary constants, and 'c' must be equal to zero."
   ]
  },
  {
   "cell_type": "markdown",
   "id": "1895467d",
   "metadata": {},
   "source": [
    "# 2. Given a recurrence relation, solve it using the substitution method:\n",
    "# d. T(n) = T(n/2) + c\n",
    "\n",
    "To solve the recurrence relation T(n) = T(n/2) + c using the substitution method:\n",
    "\n",
    "Let's assume T(n) = an + b, where 'a' and 'b' are constants to be determined.\n",
    "\n",
    "\n",
    "Substituting this assumed form into the recurrence relation:\n",
    "\n",
    "an + b = a(n/2) + b + c\n",
    "\n",
    "an + b = (a/2)n + b + c\n",
    "\n",
    "Rearranging terms:\n",
    "\n",
    "(a/2)n = c\n",
    "\n",
    "a = 2c/n\n",
    "\n",
    "This implies that 'a' must be equal to 2c/n for the equation to hold.\n",
    "\n",
    "Substituting a = 2c/n back into our assumed form of the solution, we get:\n",
    "\n",
    "T(n) = (2c/n)n + b\n",
    "\n",
    "T(n) = 2c + b\n",
    "\n",
    "Now, let's verify this solution by induction.\n",
    "\n",
    "Base Case:\n",
    "For n = 1:\n",
    "T(1) = 2c + b\n",
    "\n",
    "Inductive Step:\n",
    "Assume that T(k) = 2c + b holds for some arbitrary k ≥ 1.\n",
    "\n",
    "Now, let's prove that T(2k) = 2c + b holds:\n",
    "T(2k) = 2c + b\n",
    "\n",
    "Thus, the assumed solution T(n) = 2c + b satisfies the recurrence relation T(n) = T(n/2) + c for all n ≥ 1.\n",
    "\n",
    "Therefore, the solution to the recurrence relation T(n) = T(n/2) + c using the substitution method is T(n) = 2c + b, where 'b' is an arbitrary constant and 'c' is the given constant in the recurrence relation."
   ]
  },
  {
   "cell_type": "markdown",
   "id": "cb30c570",
   "metadata": {},
   "source": [
    "# 3. Given a recurrence relation, solve it using the recursive tree approach:\n",
    "# a. T(n) = 2T(n-1) +1\n",
    "\n",
    "\n",
    "To solve the recurrence relation T(n) = 2T(n-1) + 1 using the recursive tree approach, we can visualize the recurrence relation with a recursion tree.\n",
    "\n",
    "The recurrence relation can be represented as follows:\n",
    "\n",
    "          T(n)\n",
    "         /    \\\n",
    "      T(n-1)   T(n-1)\n",
    "       / \\      / \\\n",
    "   T(n-2) T(n-2) T(n-2) T(n-2)\n",
    "    / \\    / \\    / \\    / \\\n",
    "T(n-3) T(n-3) T(n-3) T(n-3) ...\n",
    "\n",
    "In this tree structure:\n",
    "\n",
    "Each node represents a value of T.\n",
    "Each level of the tree represents a specific value of n, where the top level represents n and subsequent levels represent n-1, n-2, and so on.\n",
    "At each level, there are two branches, representing the two recursive calls in the recurrence relation T(n) = 2T(n-1) + 1.\n",
    "Now, let's analyze the number of nodes at each level of the tree:\n",
    "\n",
    "At level 0 (top level), there is 1 node representing T(n).\n",
    "At level 1, there are 2 nodes representing T(n-1).\n",
    "At level 2, there are 4 nodes representing T(n-2).\n",
    "At level i, there are 2^i nodes representing T(n-i).\n",
    "Therefore, the total number of nodes in the tree (or the total number of function calls) is 2^0 + 2^1 + 2^2 + ... + 2^(n-1).\n",
    "\n",
    "This is a geometric series, and its sum can be calculated using the formula for the sum of a geometric series:\n",
    "\n",
    "S = a(1 - r^n) / (1 - r)\n",
    "\n",
    "where:\n",
    "\n",
    "a = 1 (the first term)\n",
    "r = 2 (the common ratio)\n",
    "n is the number of terms (or levels in the tree)\n",
    "Substituting the values into the formula, we get:\n",
    "\n",
    "S = (1(1 - 2^n)) / (1 - 2)\n",
    "\n",
    "S = 2^n - 1\n",
    "\n",
    "Therefore, the total number of function calls (or the total number of nodes in the tree) is 2^n - 1.\n",
    "\n",
    "Hence, the time complexity of the recurrence relation T(n) = 2T(n-1) + 1 using the recursive tree approach is O(2^n)."
   ]
  },
  {
   "cell_type": "markdown",
   "id": "407aeb03",
   "metadata": {},
   "source": [
    "# 3. Given a recurrence relation, solve it using the recursive tree approach:\n",
    "# b. T(n) = 2T(n/2) + n\n",
    "\n",
    "To solve the recurrence relation T(n) = 2T(n/2) + n using the recursive tree approach, we can visualize the recurrence relation with a recursion tree.\n",
    "\n",
    "The recurrence relation can be represented as follows:\n",
    "\n",
    "                    T(n)\n",
    "                 /         \\\n",
    "            T(n/2)       T(n/2)\n",
    "           /     \\       /     \\\n",
    "      T(n/4)  T(n/4) T(n/4)  T(n/4)\n",
    "       .         .      .       .\n",
    "       .         .      .       .\n",
    "       .         .      .       .\n",
    "\n",
    "\n",
    "In this tree structure:\n",
    "\n",
    "Each node represents a value of T.\n",
    "Each level of the tree represents a specific value of n, where the top level represents n and subsequent levels represent n/2, n/4, and so on.\n",
    "At each level, there are two branches, representing the two recursive calls in the recurrence relation T(n) = 2T(n/2) + n.\n",
    "Now, let's analyze the number of nodes at each level of the tree:\n",
    "\n",
    "At level 0 (top level), there is 1 node representing T(n).\n",
    "At level 1, there are 2 nodes representing T(n/2).\n",
    "At level 2, there are 4 nodes representing T(n/4).\n",
    "At level i, there are 2^i nodes representing T(n/2^i).\n",
    "Therefore, the total number of nodes in the tree (or the total number of function calls) is 2^0 + 2^1 + 2^2 + ... + 2^(log n).\n",
    "\n",
    "This is a geometric series, and its sum can be calculated using the formula for the sum of a geometric series:\n",
    "\n",
    "S = a(1 - r^(log n+1)) / (1 - r)\n",
    "\n",
    "where:\n",
    "\n",
    "a = 1 (the first term)\n",
    "r = 2 (the common ratio)\n",
    "n is the number of terms (or levels in the tree)\n",
    "Substituting the values into the formula, we get:\n",
    "\n",
    "S = (1 - 2^(log n+1)) / (1 - 2)\n",
    "\n",
    "Simplified:\n",
    "S = 2n - 1\n",
    "\n",
    "Therefore, the total number of function calls (or the total number of nodes in the tree) is 2n - 1.\n",
    "\n",
    "Hence, the time complexity of the recurrence relation T(n) = 2T(n/2) + n using the recursive tree approach is O(n)."
   ]
  },
  {
   "cell_type": "code",
   "execution_count": null,
   "id": "02cdcd97",
   "metadata": {},
   "outputs": [],
   "source": []
  }
 ],
 "metadata": {
  "kernelspec": {
   "display_name": "Python 3 (ipykernel)",
   "language": "python",
   "name": "python3"
  },
  "language_info": {
   "codemirror_mode": {
    "name": "ipython",
    "version": 3
   },
   "file_extension": ".py",
   "mimetype": "text/x-python",
   "name": "python",
   "nbconvert_exporter": "python",
   "pygments_lexer": "ipython3",
   "version": "3.11.4"
  }
 },
 "nbformat": 4,
 "nbformat_minor": 5
}
